end2end/src/end2end/End2EndPipeline.v
@@ -62,6 +62,8 @@ refine (@KamiRiscvWordProperties.kami_word_riscv_ok 5 _ _).
 all: cbv; congruence.
 Qed.
 
+(* TODO these definitions should be in KamiRiscv.v: *)
+
 Definition kami_mem_contains_bytes(bs: list Coq.Init.Byte.byte){memSizeLg}(from: Utility.word)
            (mem: Syntax.Vec (Syntax.ConstT (Syntax.Bit MemTypes.BitsPerByte)) memSizeLg): Prop :=
   forall b n,
@@ -70,9 +72,42 @@ Definition kami_mem_contains_bytes(bs: list Coq.Init.Byte.byte){memSizeLg}(from:
     = Semantics.evalConstT (Syntax.ConstVector mem)
                            (Semantics.evalZeroExtendTrunc memSizeLg (Word.wplus from (Word.natToWord _ n))).
 
+Section Move.
+  Context {mem: map.map Utility.word byte}.
+  Context (memSizeLg: Z).
+  Context (memInit: Syntax.Vec (Syntax.ConstT (Syntax.Bit MemTypes.BitsPerByte))
+                               (Z.to_nat memSizeLg)).
+
+  Definition get_kamiMemInit(n: nat): Byte.byte :=
+    byte.of_Z (Kami.Lib.Word.uwordToZ
+                 (Kami.Semantics.evalConstT (kamiMemInit _ memInit) (Kami.Lib.Word.natToWord _ n))).
+
+  Definition riscvMemInit_range(from len: nat): mem := map.of_list (List.map
+    (fun i : nat => (word.of_Z (Z.of_nat i), get_kamiMemInit i))
+    (seq from len)).
+
+  Definition riscvMemInit_values(from len: nat): list byte :=
+    List.map get_kamiMemInit (seq from len).
+
+  Definition riscvMemInit: mem := riscvMemInit_range 0 (2 ^ Z.to_nat memSizeLg).
+End Move.
+
+(* TODO remove once moved to KamiRiscv.v *)
+Goal @riscvMemInit = @KamiRiscv.riscvMemInit. Proof. reflexivity. Qed.
+
 Section Connect.
 
-  Context (instrMemSizeLg memSizeLg: Z).
+  Context (instrMemSizeLg memSizeLg stack_size_in_bytes: Z).
+
+  Definition ml: MemoryLayout := {|
+    code_start := word.of_Z 0;
+    code_pastend := word.of_Z (2 ^ (2 + instrMemSizeLg));
+    heap_start := word.of_Z (2 ^ (2 + instrMemSizeLg));
+    heap_pastend := word.of_Z (2 ^ memSizeLg - stack_size_in_bytes);
+    stack_start := word.of_Z (2 ^ memSizeLg - stack_size_in_bytes);
+    stack_pastend := word.of_Z (2 ^ memSizeLg);
+  |}.
+
   Context (memInit: Syntax.Vec (Syntax.ConstT (Syntax.Bit MemTypes.BitsPerByte))
                                (Z.to_nat memSizeLg)).
 
@@ -96,6 +131,11 @@ Section Connect.
     - exact (@KamiWord.wordWok _ (or_introl eq_refl)).
     - exact SortedListString.ok.
   Defined.
+
+  Add Ring wring : (word.ring_theory (word := Utility.word))
+      (preprocess [autorewrite with rew_word_morphism],
+       morphism (word.ring_morph (word := Utility.word)),
+       constants [word_cst]).
 
   Goal True.
   epose (_ : PrimitivesParams (MinimalMMIO.free MetricMinimalMMIO.action MetricMinimalMMIO.result)
@@ -154,15 +194,52 @@ Section Connect.
   Notation strname_sem := (FlattenExpr.mk_Semantics_params
                              (@Pipeline.FlattenExpr_parameters pipeline_params)).
   Context (spec: @ProgramSpec strname_sem)
-          (ml: MemoryLayout)
-          (mlOk: MemoryLayoutOk ml)
           (funimplsList: list (string * (list string * list string * cmd))).
 
-  Hypothesis instrMemSizeLg_agrees_with_ml:
-    word.sub ml.(code_pastend) ml.(code_start) = word.of_Z (2 ^ (2 + instrMemSizeLg)).
   Hypothesis heap_start_agree: spec.(datamem_start) = ml.(heap_start).
   Hypothesis heap_pastend_agree: spec.(datamem_pastend) = ml.(heap_pastend).
-  Hypothesis code_at_0: ml.(code_start) = word.of_Z 0.
+  Hypothesis stack_size_div: stack_size_in_bytes mod bytes_per_word = 0.
+  Hypothesis stack_size_bounds: 0 <= stack_size_in_bytes <= 2 ^ memSizeLg - 2 ^ (2 + instrMemSizeLg).
+
+  Lemma mlOk: MemoryLayoutOk ml.
+  Proof.
+    constructor;
+      unfold ml, code_start, code_pastend, heap_start, heap_pastend, stack_start, stack_pastend.
+    - reflexivity.
+    - rewrite word.unsigned_of_Z.
+      unfold word.wrap.
+      etransitivity. 1: exact (mod_2width_mod_bytes_per_word (2 ^ memSizeLg - stack_size_in_bytes)).
+      change bytes_per_word with 4.
+      apply mod4_0.mod4_0_sub.
+      + replace memSizeLg with (memSizeLg - 2 + 2) by blia.
+        rewrite Z.pow_add_r by blia.
+        apply mod4_0.mod4_mul4_r.
+      + exact stack_size_div.
+    - rewrite word.unsigned_of_Z.
+      unfold word.wrap.
+      etransitivity. 1: exact (mod_2width_mod_bytes_per_word (2 ^ memSizeLg)).
+      replace memSizeLg with (memSizeLg - 2 + 2) by blia.
+      rewrite Z.pow_add_r by blia.
+      apply mod4_0.mod4_mul4_r.
+    - rewrite word.unsigned_of_Z. change (word.wrap 0) with 0.
+      eapply proj1. eapply word.unsigned_range.
+    - reflexivity.
+    - rewrite ?word.unsigned_of_Z. unfold word.wrap.
+      pose proof (Z.pow_nonneg 2 (2 + instrMemSizeLg)).
+      change width with 32 in *.
+      assert (2 ^ memSizeLg < 2 ^ 32). {
+        apply Z.pow_lt_mono_r; blia.
+      }
+      rewrite ?Z.mod_small; try split; try apply Z.pow_nonneg; try blia.
+    - reflexivity.
+    - rewrite ?word.unsigned_of_Z. unfold word.wrap.
+      pose proof (Z.pow_nonneg 2 (2 + instrMemSizeLg)).
+      change width with 32 in *.
+      assert (2 ^ memSizeLg < 2 ^ 32). {
+        apply Z.pow_lt_mono_r; blia.
+      }
+      rewrite ?Z.mod_small; try split; try apply Z.pow_nonneg; try blia.
+    Qed.
 
   Hypothesis funimplsList_NoDup: NoDup (List.map fst funimplsList).
 
@@ -171,9 +248,6 @@ Section Connect.
      will be transformed into "exists suffix, ..." form later *)
   Definition goodTraceE(t: list Event): Prop :=
     exists bedrockTrace, traces_related t bedrockTrace /\ spec.(goodTrace) bedrockTrace.
-
-  (* Definition kamiMemToBedrockMem: mem := *)
-  (*   projT1 (riscvMemInit memInit). *)
 
   Definition bedrock2Inv := (fun t m l => forall mc, hl_inv spec t m l mc).
 
@@ -269,20 +343,22 @@ Section Connect.
       + assumption.
       + assumption.
       + assumption.
-      + move ml at bottom.
-        pose proof (mem_ok : @map.ok (@Semantics.word strname_sem) byte (@Semantics.mem strname_sem)).
+      + pose proof (mem_ok : @map.ok (@Semantics.word strname_sem) byte (@Semantics.mem strname_sem)).
         pose proof word.eqb_spec.
         cbv [imem mem_available].
 
         eapply Proper_iff1_iff1; [|reflexivity..|].
         { progress repeat rewrite ?sep_ex1_r, ?sep_ex1_l; reflexivity. }
-        eexists ?[stack].
+        exists (riscvMemInit_values _ memInit (Z.to_nat (2 ^ memSizeLg - stack_size_in_bytes))
+                                              (Z.to_nat stack_size_in_bytes)).
+         eapply Proper_iff1_iff1; [|reflexivity..|].
+        { progress repeat rewrite ?sep_ex1_r, ?sep_ex1_l; reflexivity. }
+        exists (riscvMemInit_values _ memInit (Z.to_nat (2 ^ (2 + instrMemSizeLg)))
+                       (Z.to_nat (2 ^ memSizeLg - stack_size_in_bytes - 2 ^ (2 + instrMemSizeLg)))).
         eapply Proper_iff1_iff1; [|reflexivity..|].
         { progress repeat rewrite ?sep_ex1_r, ?sep_ex1_l; reflexivity. }
-        eexists ?[heap].
-        eapply Proper_iff1_iff1; [|reflexivity..|].
-        { progress repeat rewrite ?sep_ex1_r, ?sep_ex1_l; reflexivity. }
-        eexists ?[unused_imem].
+        exists (riscvMemInit_values _ memInit (Datatypes.length (instrencode instrs))
+                       (Z.to_nat (2 ^ (2 + instrMemSizeLg)) - (Datatypes.length (instrencode instrs)))).
         eapply Proper_iff1_iff1; [|reflexivity..|].
         { progress repeat rewrite ?sep_emp_2, ?sep_emp_l, ?sep_emp_r; reflexivity. }
         eapply sep_emp_l; split.
@@ -295,23 +371,15 @@ Section Connect.
         Unshelve.
         all : case TODO_initmem .
 
-      + setoid_rewrite code_at_0.
-        assert (Hend: code_pastend ml = word.of_Z (2 ^ (2 + instrMemSizeLg))).
-        { setoid_rewrite code_at_0 in instrMemSizeLg_agrees_with_ml.
-          cbv [word.sub word.of_Z Utility.word Words32 MMIO.word mmio_params
-                        KamiWord.word kofZ]
-            in instrMemSizeLg_agrees_with_ml.
-          setoid_rewrite <-instrMemSizeLg_agrees_with_ml.
-          rewrite Word.wminus_def, Word.wplus_comm, Word.wplus_unit; trivial.
-        }
+      + change (word.unsigned (code_start ml)) with 0.
+        assert (Hend: code_pastend ml = word.of_Z (2 ^ (2 + instrMemSizeLg))) by reflexivity.
         setoid_rewrite Hend.
-        rewrite word.unsigned_of_Z_0.
         rewrite word.unsigned_of_Z.
         cbv [word.wrap].
         rewrite Z.mod_small by (split; [apply Z.pow_nonneg; Lia.lia
                                        |apply Z.pow_lt_mono_r; cbn; Lia.lia]).
         assumption.
-      + symmetry. exact code_at_0.
+      + reflexivity.
       + reflexivity.
       + unfold FlatToRiscvCommon.regs_initialized. intros.
         match goal with
